hpaxos_safety.thy
@@ -1942,4 +1942,111 @@ next
 qed
 
 
+
+lemma next_known_msgs_acc_preserved:
+  assumes "Next st st2"
+      and "x \<in> set (known_msgs_acc st a)"
+  shows "x \<in> set (known_msgs_acc st2 a)"
+proof -
+  have css: "ProposerSendAction st st2 \<or>
+        (\<exists>A :: Acceptor. is_safe A
+                    \<and> queued_msg st A = None 
+                    \<and> (\<exists>m \<in> set (msgs st). Process1a A m st st2)) \<or>
+        (\<exists>A :: Acceptor. is_safe A
+                      \<and> queued_msg st A \<noteq> None 
+                      \<and> Process1b A (the (queued_msg st A)) st st2) \<or>
+        (\<exists>A :: Acceptor. is_safe A
+                      \<and> queued_msg st A = None 
+                      \<and> (\<exists>m \<in> set (msgs st). Process1b A m st st2)) \<or>
+        (\<exists>A :: Acceptor. is_safe A
+                      \<and> two_a_lrn_loop st A 
+                      \<and> (\<exists>l :: Learner. Process1bLearnerLoopStep A l st st2)) \<or>
+        (\<exists>A :: Acceptor. is_safe A
+                      \<and> two_a_lrn_loop st A 
+                      \<and> Process1bLearnerLoopDone A st st2) \<or>
+        LearnerAction st st2 \<or>
+        (\<exists>A :: Acceptor. \<not> (is_safe A)
+                      \<and> FakeSend1b A st st2) \<or>
+        (\<exists>A :: Acceptor. \<not> (is_safe A)
+                      \<and> FakeSend2a A st st2)
+        "
+        using assms next_split by presburger
+    then show ?thesis
+    proof (elim disjE)
+      assume "ProposerSendAction st st2"
+      then show ?thesis
+        using assms(2) by auto
+    next
+      assume "\<exists>A. is_safe A \<and>
+                queued_msg st A = None \<and>
+                (\<exists>m\<in>set (msgs st).
+                    Process1a A m st st2)"
+      show ?thesis
+        by (metis Process1a.elims(2) Store_acc.elims(2) \<open>\<exists>A. is_safe A \<and> queued_msg st A = None \<and> (\<exists>m\<in>set (msgs st). Process1a A m st st2)\<close> assms(2) in_set_member member_rec(1))
+    next
+      assume "\<exists>A :: Acceptor. is_safe A
+                        \<and> queued_msg st A \<noteq> None 
+                        \<and> Process1b A (the (queued_msg st A)) st st2"
+      then show ?thesis
+      proof -
+        show ?thesis
+          using \<open>\<exists>A. is_safe A \<and> queued_msg st A \<noteq> None \<and> Process1b A (the (queued_msg st A)) st st2\<close> assms(2) by force
+      qed
+    next
+      assume "\<exists>A :: Acceptor. is_safe A
+                  \<and> queued_msg st A = None 
+                  \<and> (\<exists>m \<in> set (msgs st). Process1b A m st st2)"
+      then show ?thesis
+      proof -
+        show ?thesis
+          using \<open>\<exists>A. is_safe A \<and> queued_msg st A = None \<and> (\<exists>m\<in>set (msgs st). Process1b A m st st2)\<close> assms(2) by fastforce
+      qed
+    next
+      assume "\<exists>A :: Acceptor. is_safe A
+                        \<and> two_a_lrn_loop st A 
+                        \<and> (\<exists>l :: Learner. Process1bLearnerLoopStep A l st st2)"
+      then show ?thesis
+        by (metis Process1bLearnerLoopStep.elims(2) Store_acc.elims(2) assms(2) list.set_intros(2))
+    next
+      assume "\<exists>A. is_safe A \<and>
+        two_a_lrn_loop st A \<and>
+        Process1bLearnerLoopDone A st st2"
+      show ?thesis
+        using \<open>\<exists>A. is_safe A \<and> two_a_lrn_loop st A \<and> Process1bLearnerLoopDone A st st2\<close> assms(2) by force
+    next
+      assume "LearnerAction st st2"
+      then show ?thesis
+        by (metis (no_types, lifting) LearnerAction.elims(2) LearnerDecide.simps LearnerRecv.elims(2) assms(2) select_convs(2) surjective update_convs(3) update_convs(8))
+    next
+      assume "\<exists>A. \<not> is_safe A \<and> FakeSend1b A st st2"
+      show ?thesis
+        by (metis FakeSend1b.elims(1) \<open>\<exists>A. \<not> is_safe A \<and> FakeSend1b A st st2\<close> assms(2) select_convs(2) surjective update_convs(1))
+    next
+      assume "\<exists>A. \<not> is_safe A \<and> FakeSend2a A st st2"
+      then show ?thesis
+        by (metis FakeSend2a.simps assms(2) select_convs(2) surjective update_convs(1))
+    qed
+qed
+
+lemma spec_known_msgs_acc_preserved:
+  assumes "Spec f"
+      and "x \<in> set (known_msgs_acc (f i) a)"
+  shows "x \<in> set (known_msgs_acc (f (i + 1)) a)"
+  by (metis Spec.elims(2) Suc_eq_plus1 assms(1) assms(2) next_known_msgs_acc_preserved)
+
+lemma known_msgs_acc_preserved:
+  assumes "Spec f"
+  shows "j \<ge> i \<longrightarrow> x \<in> set (known_msgs_acc (f i) a) \<longrightarrow> x \<in> set (known_msgs_acc (f j) a)"
+proof (induction j)
+  case 0
+  then show ?case
+    by simp
+next
+  case (Suc j)
+  then show ?case
+    by (metis One_nat_def add.right_neutral add_Suc_right assms le_SucE spec_known_msgs_acc_preserved)
+qed
+
+
+
 end
